proved thms for empty deduction relation

src/tools/parallelcomposition/derived_rules_emptydeductionScript.sml
@@ -12,9 +12,12 @@ val traces_def =
 Define`
       traces ((MTrn:('event, 'pred, 'state, 'symb) mtrel),(ded:('pred) tded)) ((Sym:'symb set),(P: 'pred set),(S: 'state)) ((Sym':'symb set),(P': 'pred set),(S': 'state)) = {t| (MTrn (Sym,P,S) t (Sym',P',S'))}
                                                                                                                                                                         `;
- val comptraces_def =
+val comptraces_def =
 Define`
-      comptraces ((CMTrn:((('event1+'eventS) + ('event2 +'eventS)), ('pred1 + 'pred2), 'state1#'state2, 'symb) mtrel),(CDed:('pred1 + 'pred2)tded)) ((Sym:'symb set),(P: ('pred1 + 'pred2) set),(S1: 'state1),(S2: 'state2)) ((Sym':'symb set),(P': ('pred1 + 'pred2) set),(S1': 'state1),(S2': 'state2)) = {t| (CMTrn (Sym,P,S1,S2) t (Sym',P',S1',S2'))}
+      comptraces ((MTrn1:('event1 + 'eventS, 'pred1, 'state1, 'symb) mtrel),(Ded1:('pred1) tded)) ((MTrn2:('event2 + 'eventS, 'pred2, 'state2, 'symb) mtrel),(Ded2:('pred2) tded)) ((Sym:'symb set),(P: ('pred1 + 'pred2) set),(S1: 'state1),(S2: 'state2)) ((Sym':'symb set),(P': ('pred1 + 'pred2) set),(S1': 'state1),(S2': 'state2)) =
+{(t: ((('event1 + 'eventS) + 'event2 + 'eventS) option list))|  
+ (((MTrn1,Ded1) || (MTrn2,Ded2)) (Sym,P,S1,S2) t (Sym',P',S1',S2'))
+}
 `;
 
 val binterleave_trace_comp_to_decomp_emptydeduction_thm = store_thm(
@@ -57,7 +60,7 @@ val binterleave_trace_comp_to_decomp_emptydeduction_thm = store_thm(
 
 val binterleave_trace_decomp_to_comp_emptydeduction_thm = store_thm(
   "binterleave_trace_decomp_to_comp_emptydeduction",
-  ``∀t Sym P S1 S2 Sym' P' S1' S2' (MTrn1:('event1 + 'eventS, 'pred1, 'state1, 'symb) mtrel) (MTrn2:('event2 + 'eventS, 'pred2, 'state2, 'symb) mtrel) Ded1 Ded2. 
+  ``∀t Sym P S1 S2 Sym' P' S1' S2' (MTrn1:('event1 + 'eventS, 'pred1, 'state1, 'symb) mtrel) (MTrn2:('event2 + 'eventS, 'pred2, 'state2, 'symb) mtrel) (Ded1:('pred1) tded) (Ded2:('pred2) tded). 
        (∃t1 t2. (MTrn1 (Sym,(IMAGE OUTL P),S1) t1 (Sym',(IMAGE OUTL P'),S1')) ∧ (MTrn2 (Sym,(IMAGE OUTR P),S2) t2 (Sym',(IMAGE OUTR P'),S2')) ∧ (binterl t1 t2 t))
      ⇒
      (((MTrn1,Ded1) || (MTrn2,Ded2)) (Sym,P,S1,S2) t (Sym',P',S1',S2'))
@@ -89,6 +92,40 @@ val binterleave_trace_decomp_to_comp_emptydeduction_thm = store_thm(
      FULL_SIMP_TAC (list_ss++pred_setSimps.PRED_SET_ss++boolSimps.LIFT_COND_ss++boolSimps.EQUIV_EXTRACT_ss) [symbolicParlComp_def] >> rpt strip_tac >> IMP_RES_TAC binterl_moveNONE >> rw[] >> IMP_RES_TAC TranRelSnocRevNone>>
      Q.EXISTS_TAC `P''` >>  rw[] >> PAT_X_ASSUM ``!Sym P S1 S2 Sym' P' S1' S2' MTrn1 MTrn2 Ded1 Ded2. A`` (ASSUME_TAC o (Q.SPECL [`Sym`,`P`,`S1`,`S2`,`Sym'`,`P''`,`S1'`,`S2'`,`MTrn1`,`MTrn2`,`Ded1`,`Ded2`])) >> IMP_RES_TAC binterl_movenone >> RES_TAC
   );
+
+
+val binterleave_trace_emptydeduction_thm = store_thm(
+  "binterleave_trace_emptydeduction", ``
+                       ∀t Sym P S1 S2 Sym' P' S1' S2' (MTrn1:('event1 + 'eventS, 'pred1, 'state1, 'symb) mtrel) (MTrn2:('event2 + 'eventS, 'pred2, 'state2, 'symb) mtrel) (Ded1:('pred1) tded) (Ded2:('pred2) tded). 
+                         (((MTrn1,Ded1) || (MTrn2,Ded2)) (Sym,P,S1,S2) t (Sym',P',S1',S2'))
+                         ⇔
+                           (∃t1 t2. (MTrn1 (Sym,(IMAGE OUTL P),S1) t1 (Sym',(IMAGE OUTL P'),S1')) ∧ (MTrn2 (Sym,(IMAGE OUTR P),S2) t2 (Sym',(IMAGE OUTR P'),S2')) ∧ (binterl t1 t2 t))
+                           ``,
+                           rpt gen_tac >> EQ_TAC >>
+                       rewrite_tac[binterleave_trace_comp_to_decomp_emptydeduction_thm] >>
+                       rewrite_tac[binterleave_trace_decomp_to_comp_emptydeduction_thm]
+  );
+
+val binterleave_composition_emptydeduction_thm = store_thm(
+  "binterleave_composition_emptydeduction", ``
+  ∀Sym P S1 S2 Sym' P' S1' S2' (MTrn1:('event1 + 'eventS, 'pred1, 'state1, 'symb) mtrel) (MTrn2:('event2 + 'eventS, 'pred2, 'state2, 'symb) mtrel) (Ded1:('pred1) tded) (Ded2:('pred2) tded).
+   (comptraces (MTrn1,Ded1) (MTrn2,Ded2) (Sym,P,S1,S2) (Sym',P',S1',S2'))                           
+  = (binterleave_ts (traces (MTrn1,Ded1) (Sym,(IMAGE OUTL P),S1) (Sym',(IMAGE OUTL P'),S1')) (traces (MTrn2,Ded2) (Sym,(IMAGE OUTR P),S2) (Sym',(IMAGE OUTR P'),S2')))
+``,
+rewrite_tac[binterleave_ts,traces_def,comptraces_def,EXTENSION] >> rw[] >> rewrite_tac[binterleave_trace_emptydeduction_thm]   
+  ); 
+  
+
+  
+val compose_vs_modules_emptydeduction_thm = store_thm(
+  "compose_vs_modules_emptydeduction_thm", ``
+                           !Sym Sym' Sym'' Sym''' P P' P'' P''' S1 S1' S1'' S1''' S2 S2' S2'' S2''' (MTrn1:('event1 + 'eventS, 'pred1, 'state1, 'symb) mtrel) (MTrn1':('event1 + 'eventS, 'pred1, 'state1, 'symb) mtrel) (MTrn2:('event2 + 'eventS, 'pred2, 'state2, 'symb) mtrel) (MTrn2':('event2 + 'eventS, 'pred2, 'state2, 'symb) mtrel) (Ded1:('pred1) tded) (Ded1':('pred1) tded) (Ded2:('pred2) tded) (Ded2':('pred2) tded).
+                             (((traces (MTrn1,Ded1) (Sym,(IMAGE OUTL P),S1) (Sym',(IMAGE OUTL P'),S1')) ⊆ (traces (MTrn1',Ded1') (Sym'',(IMAGE OUTL P''),S1'') (Sym''',(IMAGE OUTL P'''),S1'''))) ∧ ((traces (MTrn2,Ded2) (Sym,(IMAGE OUTR P),S2) (Sym',(IMAGE OUTR P'),S2')) ⊆ (traces (MTrn2',Ded2') (Sym'',(IMAGE OUTR P''),S2'') (Sym''',(IMAGE OUTR P'''),S2''')))
+                             ) ==> ((comptraces (MTrn1,Ded1) (MTrn2,Ded2) (Sym,P,S1,S2) (Sym',P',S1',S2')) ⊆ (comptraces (MTrn1',Ded1') (MTrn2',Ded2') (Sym'',P'',S1'',S2'') (Sym''',P''',S1''',S2'''))) ``
+  ,
+  rewrite_tac[binterleave_composition_emptydeduction_thm,binterleave_ts] >>
+  FULL_SIMP_TAC (list_ss++pred_setSimps.PRED_SET_ss++boolSimps.LIFT_COND_ss++boolSimps.EQUIV_EXTRACT_ss) [SUBSET_DEF] >> metis_tac[]
+  );  
 
 
 
