src/tools/parallelcomposition/interleavingScript.sml
@@ -163,7 +163,7 @@ rewrite_tac[binterleave_ts,traces_def,comptraces_def,EXTENSION] >> rw[] >> rewri
 
 val compose_vs_modules_thm = store_thm(
   "compose_vs_modules_thm", ``
-                           !Sym Sym' Sym'' Sym''' P P' P'' P''' S1 S1' S1'' S1''' S2 S2' S2'' S2''' (MTrn1:('event1 + 'eventS, 'pred1, 'state1, 'symb) mtrel) (MTrn1':('event1 + 'eventS, 'pred1, 'state1, 'symb) mtrel) (MTrn1':('event1 + 'eventS, 'pred1, 'state1, 'symb) mtrel) (MTrn1':('event1 + 'eventS, 'pred1, 'state1, 'symb) mtrel) (MTrn2:('event1 + 'eventS, 'pred1, 'state1, 'symb) mtrel) (MTrn:('event2 + 'eventS, 'pred2, 'state2, 'symb) mtrel) (MTrn2':('event1 + 'eventS, 'pred1, 'state1, 'symb) mtrel) (MTrn:('event2 + 'eventS, 'pred2, 'state2, 'symb) mtrel) Ded1 Ded1' Ded2 Ded2'.
+                          !Sym Sym' Sym'' Sym''' P P' P'' P''' S1 S1' S1'' S1''' S2 S2' S2'' S2''' (MTrn1:('event1 + 'eventS, 'pred1, 'state1, 'symb) mtrel) (MTrn1':('event1 + 'eventS, 'pred1, 'state1, 'symb) mtrel) (MTrn2:('event2 + 'eventS, 'pred2, 'state2, 'symb) mtrel) (MTrn2':('event2 + 'eventS, 'pred2, 'state2, 'symb) mtrel) (Ded1:('pred1) tded) (Ded1':('pred1) tded) (Ded2:('pred2) tded) (Ded2':('pred2) tded).
                              (((traces MTrn1 (Sym,(IMAGE OUTL P),S1) (Sym',(IMAGE OUTL P'),S1')) ⊆ (traces MTrn1' (Sym'',(IMAGE OUTL P''),S1'') (Sym''',(IMAGE OUTL P'''),S1'''))) ∧ ((traces MTrn2 (Sym,(IMAGE OUTR P),S2) (Sym',(IMAGE OUTR P'),S2')) ⊆ (traces MTrn2' (Sym'',(IMAGE OUTR P''),S2'') (Sym''',(IMAGE OUTR P'''),S2''')))
                              ) ==> ((comptraces (FST((MTrn1,Ded1) || (MTrn2,Ded2))) (Sym,P,S1,S2) (Sym',P',S1',S2')) ⊆ (comptraces (FST((MTrn1',Ded1') || (MTrn2',Ded2'))) (Sym'',P'',S1'',S2'') (Sym''',P''',S1''',S2'''))) ``
   ,
